Adapted from CPDT a reflective solver for propositional logic. Cleaned up CMon and CMon2 in terms of naming, code ordering etc. Added tests to all three of these.

Reification/CMon.v
@@ -1,12 +1,6 @@
 Add Rec LoadPath "/home/zeimer/Code/Coq".
 
-Require Import Arith.
-Require Import Permutation.
-Require Import Perm.
-Require Import InsertionSort.
-
-Require Import List.
-Import ListNotations.
+Require Import ReificationBase.
 
 Set Implicit Arguments.
 
@@ -32,10 +26,10 @@ Arguments Id [X].
 Arguments Var [X] _.
 Arguments Op [X] _ _.
 
-Fixpoint expDenote {X : CMon} (env : nat -> X) (e : exp X) : X :=
+Fixpoint expDenote {X : CMon} (env : Env X) (e : exp X) : X :=
 match e with
     | Id => neutr
-    | Var n => env n
+    | Var n => nth n env neutr
     | Op e1 e2 => op (expDenote env e1) (expDenote env e2)
 end.
 
@@ -52,33 +46,38 @@ match e with
 end.
 
 Theorem simplifyExp_correct :
-  forall (X : CMon) (env : nat -> X) (e : exp X),
+  forall (X : CMon) (env : Env X) (e : exp X),
     expDenote env (simplifyExp e) = expDenote env e.
 Proof.
-  induction e; cbn.
-    reflexivity.
-    reflexivity.
-    destruct (simplifyExp e1), (simplifyExp e2); cbn in *;
-      rewrite <- ?IHe1, <- ?IHe2, ?neutr_l, ?neutr_r; try reflexivity.
-Restart.
   intros. functional induction simplifyExp e; cbn;
   rewrite <- ?IHe, <- ?IHe0, <- ?IHe1, ?e3, ?e4; cbn;
   rewrite ?neutr_l, ?neutr_r; trivial.
 Qed.
 
-Fixpoint expDenoteL {X : CMon} (env : nat -> X) (l : list nat) : X :=
+Fixpoint expDenoteL {X : CMon} (env : Env X) (l : list nat) : X :=
 match l with
     | [] => neutr
-    | h :: t => op (env h) (expDenoteL env t)
+    | h :: t => op (nth h env neutr) (expDenoteL env t)
 end.
 
 Lemma expDenoteL_app :
-  forall (X : CMon) (env : nat -> X) (l1 l2 : list nat),
+  forall (X : CMon) (env : Env X) (l1 l2 : list nat),
     expDenoteL env (l1 ++ l2) = op (expDenoteL env l1) (expDenoteL env l2).
 Proof.
   induction l1 as [| h1 t1]; simpl; intros.
     rewrite neutr_l. reflexivity.
     rewrite <- assoc, IHt1. reflexivity.
+Qed.
+
+Lemma expDenoteL_Permutation :
+  forall (X : CMon) (env : Env X) (l1 l2 : list nat),
+    Permutation l1 l2 -> expDenoteL env l1 = expDenoteL env l2.
+Proof.
+  induction 1; cbn.
+    reflexivity.
+    rewrite IHPermutation. reflexivity.
+    rewrite !assoc. rewrite (comm (nth y env neutr)). reflexivity.
+    rewrite IHPermutation1, IHPermutation2. reflexivity.
 Qed.
 
 Fixpoint flatten {X : CMon} (e : exp X) : list nat :=
@@ -89,7 +88,7 @@ match e with
 end.
 
 Theorem flatten_correct :
-  forall (X : CMon) (env : nat -> X) (e : exp X),
+  forall (X : CMon) (env : Env X) (e : exp X),
     expDenoteL env (flatten e) = expDenote env e.
 Proof.
   induction e; simpl.
@@ -98,19 +97,8 @@ Proof.
     rewrite expDenoteL_app. rewrite IHe1, IHe2. reflexivity.
 Qed.
 
-Lemma expDenoteL_Permutation :
-  forall (X : CMon) (env : nat -> X) (l1 l2 : list nat),
-    Permutation l1 l2 -> expDenoteL env l1 = expDenoteL env l2.
-Proof.
-  induction 1; cbn.
-    reflexivity.
-    rewrite IHPermutation. reflexivity.
-    rewrite !assoc. rewrite (comm (env y)). reflexivity.
-    rewrite IHPermutation1, IHPermutation2. reflexivity.
-Qed.
-
 Theorem sort_correct :
-  forall (X : CMon) (env : nat -> X) (l : list nat) (s : Sort),
+  forall (X : CMon) (env : Env X) (l : list nat) (s : Sort),
     expDenoteL env (s natle l) = expDenoteL env l.
 Proof.
   intros. apply expDenoteL_Permutation. apply (perm_Permutation natle).
@@ -121,314 +109,88 @@ Definition simplify {X : CMon} (e : exp X) : list nat :=
   insertionSort natle (flatten (simplifyExp e)).
 
 Theorem simplify_correct :
-  forall (X : CMon) (env : nat -> X) (e1 e2 : exp X),
+  forall (X : CMon) (env : Env X) (e : exp X),
+    expDenoteL env (simplify e) = expDenote env e.
+Proof.
+  unfold simplify. intros.
+  rewrite !(sort_correct _ _ _ Sort_insertionSort).
+  rewrite !flatten_correct, !simplifyExp_correct.
+  trivial.
+Qed.
+
+Theorem reflectEq :
+  forall (X : CMon) (env : Env X) (e1 e2 : exp X),
     expDenoteL env (simplify e1) = expDenoteL env (simplify e2) ->
       expDenote env e1 = expDenote env e2.
 Proof.
-  unfold simplify. intros.
-  rewrite !(sort_correct X env _ Sort_insertionSort) in H.
-  rewrite !flatten_correct, !simplifyExp_correct in H.
-  assumption.
+  intros. rewrite !simplify_correct in H. assumption.
 Qed.
 
-Ltac inList x l :=
-match l with
-    | [] => false
-    | x :: _ => true
-    | _ :: ?l' => inList x l'
-end.
-
-Ltac addToList x l :=
-  let b := inList x l in
-match b with
-    | true => l
-    | false => constr:(x :: l)
-end.
-
-Ltac lookup x l :=
-match l with
-    | x :: _ => constr:(0)
-    | _ :: ?l' => let n := lookup x l' in constr:(S n)
-end.
-
-Ltac allVars xs e :=
+Ltac allVarsExp xs e :=
 match e with
     | op ?e1 ?e2 =>
-        let xs' := allVars xs e2 in allVars xs' e1
-    | ?f ?e' => allVars xs e'
+        let xs' := allVarsExp xs e2 in allVarsExp xs' e1
     | _ => addToList e xs
 end.
 
-Ltac reifyTerm env x :=
+Ltac reifyExp env x :=
 match x with
     | neutr => constr:(Id)
     | op ?a ?b =>
-        let e1 := reifyTerm env a in
-        let e2 := reifyTerm env b in constr:(Op e1 e2)
+        let e1 := reifyExp env a in
+        let e2 := reifyExp env b in constr:(Op e1 e2)
     | _ =>
         let n := lookup x env in constr:(Var n)
 end.
 
-Ltac functionalize l X :=
-let rec loop n l' :=
-    match l' with
-        | [] => constr:(fun _ : nat => @neutr X)
-        | ?h :: ?t =>
-            let f := loop (S n) t in
-            constr:(fun m : nat => if m =? n then h else f m)
-    end
-in loop 0 l.
+Ltac reifyEq env a b :=
+    let e1 := reifyExp env a in
+    let e2 := reifyExp env b in
+      constr:(expDenote env e1 = expDenote env e2).
 
-Ltac reify X :=
+Ltac reflectGoal' := cbn; intros; subst;
 match goal with
-    | |- ?e1 = ?e2 =>
-        let xs := allVars constr:(@nil X) e1 in
-        let xs' := allVars xs e2 in
-        let r1 := reifyTerm xs' e1 in
-        let r2 := reifyTerm xs' e2 in
-        let env := functionalize xs' X in
-        change (expDenote env r1 = expDenote env r2)
+    | X : CMon |- ?a = ?b =>
+        let xs := allVarsExp constr:(@nil X) b in
+        let xs' := allVarsExp xs a in
+        let e := reifyEq xs' a b in
+          change e; apply reflectEq; cbn; rewrite ?neutr_l, ?neutr_r
 end.
 
-Ltac reifyEqv X env a b :=
-    let e1 := reifyTerm env a in
-    let e2 := reifyTerm env b in constr:((e1, e2)).
+Ltac reflectGoal := reflectGoal; reflexivity.
 
-(* TODO : improve reflection *)
-Theorem flat_reflect_goal :
-  forall (X : CMon) (env : nat -> X) (e1 e2 : exp X),
-    flatten (simplifyExp e1) = flatten (simplifyExp e2) ->
-      expDenote env e1 = expDenote env e2.
+Section Test.
+
+Variable (X : CMon) (a a' b b' c c' d e f : X).
+
+(* [CMon] axioms. *)
+Goal op a (op b c) = op (op a b) c.
+Proof. reflectGoal'. reflexivity. Qed.
+
+Goal op neutr a = a.
+Proof. reflectGoal'. reflexivity. Qed.
+
+Goal op a neutr = a.
+Proof. reflectGoal'. reflexivity. Qed.
+
+Goal op a b = op b a.
+Proof. reflectGoal'. reflexivity. Qed.
+
+Goal op a (op (op b c) (op d (op (op e e) d))) =
+     op (op a d) (op d (op c (op e (op e b)))).
+Proof. reflectGoal'. reflexivity. Qed.
+
+(* Other tests. *)
+Goal b = b' -> op a (op b c) = op (op a b') c.
+Proof. reflectGoal'. reflexivity. Qed.
+
+Goal op a b = op a b' -> op (op a b) c = op b' (op a c).
 Proof.
-  intros. apply simplify_correct. unfold simplify. rewrite H. reflexivity.
+  reflectGoal'. rewrite ?assoc. rewrite (comm b').
+  rewrite <- !H. reflectGoal'. reflexivity.
 Qed.
 
-Theorem flat_reflect_hyp' :
-  forall (X : CMon) (env : nat -> X) (e1 e2 : exp X) (s : Sort),
-    expDenote env e1 = expDenote env e2 ->
-      expDenoteL env (s natle (flatten (simplifyExp e1))) =
-      expDenoteL env (s natle (flatten (simplifyExp e2))).
-Proof.
-  intros.
-  rewrite !sort_correct, !flatten_correct, !simplifyExp_correct.
-  assumption.
-Qed.
+Goal a = b -> b = c -> c = a -> op b (op a c) = op a (op neutr (op b c)).
+Proof. reflectGoal'. reflexivity. Qed.
 
-Ltac cmon_subst := repeat
-multimatch goal with
-    | H : ?x = ?y |- _ => rewrite <- ?H in *
-    | H : ?x = ?x |- _ => clear H
-end.
-
-Ltac reflect_cmon' := cbn; intros; cmon_subst;
-match goal with
-    | X : CMon |- ?e1 = ?e2 =>
-        reify X; apply simplify_correct; cbn; rewrite ?neutr_l, ?neutr_r
-end.
-
-Ltac reflect_cmon := reflect_cmon'; try reflexivity.
-
-Ltac reflect_goal := simpl; intros;
-match goal with
-    | X : CMon |- ?e1 = ?e2 =>
-        reify X; apply flat_reflect_goal
-end.
-
-Goal forall (X : CMon) (a b c : X),
-  op a (op b c) = op (op a b) c.
-Proof.
-  reflect_cmon.
-Qed.
-
-Goal forall (X : CMon) (a b : X),
-  op a b = op b a.
-Proof.
-  reflect_cmon.
-Qed.
-
-Goal forall (X : CMon) (a b b' c : X),
-  b = b' -> op a (op b c) = op (op a b') c.
-Proof.
-  reflect_cmon'. reflexivity.
-Qed.
-
-Goal forall (X : CMon) (a a' b b' c c' : X),
-  op a b = op a b' -> op (op a b) c = op b' (op a c).
-Proof.
-  reflect_cmon'. rewrite ?assoc. rewrite (comm b').
-  rewrite !H. reflect_cmon'. reflexivity.
-Qed.
-
-Goal forall (X : CMon) (a a' b b' c c' : X),
-  a = b -> b = c -> c = a -> op b (op a c) = op a (op neutr (op b c)).
-Proof.
-  reflect_cmon'. reflexivity.
-Qed.
-
-Inductive formula (X : CMon) : Type :=
-    | fVar : Prop -> formula X
-    | fEquiv : exp X -> exp X -> formula X
-    | fNot : formula X -> formula X
-    | fAnd : formula X -> formula X -> formula X
-    | fOr : formula X -> formula X -> formula X
-    | fImpl : formula X -> formula X -> formula X.
-
-Fixpoint formulaDenote {X : CMon} (env : nat -> X) (p : formula X)
-  : Prop :=
-match p with
-    | fVar P => P
-    | fEquiv e1 e2 => expDenote env e1 = expDenote env e2
-    | fNot p' => ~ formulaDenote env p'
-    | fAnd p1 p2 => formulaDenote env p1 /\ formulaDenote env p2
-    | fOr p1 p2 => formulaDenote env p1 \/ formulaDenote env p2
-    | fImpl p1 p2 => formulaDenote env p1 -> formulaDenote env p2
-end.
-
-Function simplifyFormula {X : CMon} (f : formula X) : formula X :=
-match f with
-    | fVar P => fVar X P
-    | fEquiv e1 e2 => fEquiv e1 e2
-    | fNot f' => fNot (simplifyFormula f')
-    | fAnd f1 f2 =>
-        match simplifyFormula f1, simplifyFormula f2 with
-            | fOr f11 f12, f2' => fOr (fAnd f11 f2') (fAnd f12 f2')
-            | f1', fOr f21 f22 => fOr (fAnd f1' f21) (fAnd f1' f22)
-            | f1', f2' => fAnd f1' f2'
-        end
-    | fOr f1 f2 =>
-        match simplifyFormula f1, simplifyFormula f2 with
-            | fAnd f11 f12, f2' => fAnd (fOr f11 f2') (fOr f12 f2')
-            | f1', fAnd f21 f22 => fAnd (fOr f1' f21) (fOr f1' f22)
-            | f1', f2' => fOr f1' f2'
-        end
-    | fImpl f1 f2 =>
-        match simplifyFormula f1 with
-            | fAnd f11 f12 => fImpl f11 (fImpl f12 f2)
-            | fOr f11 f12 => fAnd (fImpl f11 f2) (fImpl f12 f2)
-            | f1' => fImpl f1' f2
-        end
-end.
-
-Theorem simplifyFormula_correct :
-  forall (X : CMon) (env : nat -> X) (f : formula X),
-    formulaDenote env (simplifyFormula f) <-> formulaDenote env f.
-Proof.
-  intros. Time functional induction simplifyFormula f; cbn;
-  repeat match goal with
-      | env : nat -> _, IH : forall env' : nat -> _, _ |- _ =>
-          specialize (IH env)
-      | e : simplifyFormula ?f = _,
-        IH : formulaDenote _ (simplifyFormula ?f) <-> _ |- _ =>
-        rewrite <- IH, e; cbn
-  end; firstorder.
-Qed.
-
-Ltac allVarsFormula xs P :=
-match P with
-    | ?a = ?b => allVars xs P
-    | ~ ?P' => allVarsFormula xs P'
-    | ?P1 /\ ?P2 =>
-        let xs' := allVarsFormula xs P1 in
-          allVarsFormula xs' P2
-    | ?P1 \/ ?P2 =>
-        let xs' := allVarsFormula xs P1 in
-          allVarsFormula xs' P2
-    | ?P1 -> ?P2 =>
-        let xs' := allVarsFormula xs P1 in
-          allVarsFormula xs' P2
-    | _ => xs
-end.
-
-Ltac reifyFormula X xs P :=
-match P with
-    | ~ ?P' =>
-        let e := reifyFormula X xs P' in constr:(fNot e)
-    | ?a = ?b =>
-        let e1 := reifyTerm xs a in
-        let e2 := reifyTerm xs b in constr:(fEquiv e1 e2)
-    | ?P1 /\ ?P2 =>
-        let e1 := reifyFormula X xs P1 in
-        let e2 := reifyFormula X xs P2 in constr:(fAnd e1 e2)
-    | ?P1 \/ ?P2 =>
-        let e1 := reifyFormula X xs P1 in
-        let e2 := reifyFormula X xs P2 in constr:(fOr e1 e2)
-    | ?P1 -> ?P2 =>
-        let e1 := reifyFormula X xs P1 in
-        let e2 := reifyFormula X xs P2 in constr:(fImpl e1 e2)
-    | _ => constr:(fVar X P)
-end.
-
-Ltac reifyGoal :=
-match goal with
-    | X : CMon |- ?P =>
-        let xs := allVarsFormula constr:(@nil X) P in
-        let env := functionalize xs X in
-        let e := reifyFormula X xs P in change (formulaDenote env e)
-end.
-
-Definition list_eq :
-  forall (l1 l2 : list nat), {l1 = l2} + {l1 <> l2}.
-Proof.
-  do 2 decide equality.
-Defined.
-
-Fixpoint solveFormula {X : CMon} (env : nat -> X) (f : formula X)
-  : option (formulaDenote env f).
-Proof.
-  destruct f; cbn.
-    apply None.
-    destruct (list_eq
-              (insertionSort natle (flatten (simplifyExp e)))
-              (insertionSort natle (flatten (simplifyExp e0)))).
-      apply Some. apply simplify_correct. f_equal. assumption.
-      apply None.
-    apply None.
-    destruct (solveFormula X env f1), (solveFormula X env f2).
-      apply Some. split; assumption.
-      1-3: apply None.
-    destruct (solveFormula X env f1).
-      apply Some. left. assumption.
-      destruct (solveFormula X env f2).
-        apply Some. right. assumption.
-        apply None.
-    destruct (solveFormula X env f2).
-      apply Some. intro. assumption.
-      apply None.
-Defined.
-
-Theorem solveFormula_spec :
-  forall (X : CMon) (env : nat -> X) (f : formula X),
-    (exists p : formulaDenote env f, solveFormula env f = Some p) ->
-      formulaDenote env f.
-Proof.
-  intros. destruct H. assumption.
-Qed.
-
-Ltac solve_goal' :=
-  cbn; intros; cmon_subst; reifyGoal;
-  apply solveFormula_spec; cbn; eauto.
-
-Ltac solve_goal :=
-  try (solve_goal'; fail);
-  fail "Cannot solve the goal".
-
-Goal forall (X : CMon) (a a' b b' c c' : X),
-  a = b -> b = c -> c = a -> a = c /\ op c c = op b b.
-Proof.
-  solve_goal.
-Qed.
-
-Goal forall (X : CMon) (a a' b b' c c' : X),
-  a = b -> b' = c' -> 2 = 2 \/ op c c = op c (op a c').
-Proof.
-  Require Import Quote.
-  intros X a _ b b' c c'.
-  match goal with
-      | X : CMon |- ?P =>
-          let xs := allVarsFormula constr:(@nil X) P in
-          let env := functionalize xs X in
-          let f := fresh "f" in
-          let f' := constr:(@formulaDenote X env) in pose f' as f
-  end; cbn in *.
-  Print formulaDenote. Print Assumptions simplify_correct.
-Abort.
+End Test.
