Reification/ReificationBase.v
@@ -1,0 +1,36 @@
+Add Rec LoadPath "/home/zeimer/Code/Coq".
+
+Require Export Arith.
+
+Require Export Permutation.
+Require Export Perm.
+Require Export InsertionSort.
+
+Require Export List.
+Export ListNotations.
+
+Require Export Equality.
+
+Set Implicit Arguments.
+
+Ltac inList x l :=
+match l with
+    | [] => false
+    | x :: _ => true
+    | _ :: ?l' => inList x l'
+end.
+
+Ltac addToList x l :=
+  let b := inList x l in
+match b with
+    | true => l
+    | false => constr:(x :: l)
+end.
+
+Ltac lookup x l :=
+match l with
+    | x :: _ => constr:(0)
+    | _ :: ?l' => let n := lookup x l' in constr:(S n)
+end.
+
+Definition Env (X : Type) : Type := list X.
